CertiGC/gc_spec.v
@@ -408,7 +408,7 @@ Definition resume_spec :=
          thread_info_rep sh t_info ti)
   POST [tvoid]
     PROP (Ptrofs.unsigned (ti_nalloc t_info) <=
-           total_space (heap_head (ti_heap t_info))
+           available_space (heap_head (ti_heap t_info))
           - used_space (heap_head (ti_heap t_info)))
     RETURN ()
     SEP (all_string_constants rsh gv;
@@ -441,7 +441,7 @@ Definition garbage_collect_spec :=
           safe_to_copy g';
           frame_shells_eq (ti_frames t_info) (ti_frames t_info');
           Ptrofs.unsigned (ti_nalloc t_info) <=
-                 total_space (heap_head (ti_heap t_info'))
+                 available_space (heap_head (ti_heap t_info'))
                     - used_space (heap_head (ti_heap t_info')))
     RETURN ()
     SEP (mem_mgr gv;
